theories/stdpp_extra.v
@@ -1,4 +1,4 @@
-From stdpp Require Import countable.
+From stdpp Require Import countable list.
 From iris.base_logic Require Import invariants.
 
 Lemma elements_list_to_set {A} `{Countable A} (l: list A) :
@@ -89,3 +89,523 @@ Proof.
   intros * HH. rewrite elem_of_disjoint. intros x.
   rewrite !elem_of_list_to_set. rewrite elem_of_disjoint in HH |- *. eauto.
 Qed.
+
+Lemma map_to_list_fst {A B : Type} `{EqDecision A, Countable A} (m : gmap A B) i :
+  i ∈ (map_to_list m).*1 ↔ (∃ x, (i,x) ∈ (map_to_list m)).
+Proof.
+  split.
+  - intros Hi.
+    destruct (m !! i) eqn:Hsome.
+    + exists b. by apply elem_of_map_to_list.
+    + rewrite -(list_to_map_to_list m) in Hsome.
+      eapply not_elem_of_list_to_map in Hsome. done.
+  - intros [x Hix].
+    apply elem_of_list_fmap.
+    exists (i,x). auto.
+Qed.
+
+Lemma drop_S':
+    forall A l n (a: A) l',
+      drop n l = a::l' ->
+      drop (S n) l = l'.
+Proof.
+  induction l; intros * HH.
+  - rewrite drop_nil in HH. inversion HH.
+  - simpl. destruct n.
+    + rewrite drop_0 in HH. inversion HH.
+      reflexivity.
+    + simpl in HH. eapply IHl; eauto.
+Qed.
+
+Lemma disjoint_nil_l {A : Type} `{EqDecision A} (a : A) (l2 : list A) :
+  [] ## l2.
+Proof.
+  apply elem_of_disjoint. intros x Hcontr. inversion Hcontr.
+Qed.
+
+Lemma disjoint_nil_r {A : Type} `{EqDecision A} (a : A) (l2 : list A) :
+  l2 ## [].
+Proof.
+  apply elem_of_disjoint. intros x Hl Hcontr. inversion Hcontr.
+Qed.
+
+Lemma disjoint_cons {A : Type} `{EqDecision A} (a : A) (l1 l2 : list A) :
+  a :: l1 ## l2 → a ∉ l2.
+Proof.
+  rewrite elem_of_disjoint =>Ha.
+  assert (a ∈ a :: l1) as Hs; [apply elem_of_cons;auto;apply elem_of_nil|].
+  specialize (Ha a Hs). done.
+Qed.
+
+Lemma disjoint_weak {A : Type} `{EqDecision A} (a : A) (l1 l2 : list A) :
+  a :: l1 ## l2 → l1 ## l2.
+Proof.
+  rewrite elem_of_disjoint =>Ha a' Hl1 Hl2.
+  assert (a' ∈ a :: l1) as Hs; [apply elem_of_cons;auto;apply elem_of_nil|].
+  specialize (Ha a' Hs Hl2). done.
+Qed.
+
+Lemma disjoint_swap {A : Type} `{EqDecision A} (a : A) (l1 l2 : list A) :
+  a ∉ l1 →
+  a :: l1 ## l2 -> l1 ## a :: l2.
+Proof.
+  rewrite elem_of_disjoint =>Hnin Ha a' Hl1 Hl2.
+  destruct (decide (a' = a)).
+  - subst. contradiction.
+  - apply Ha with a'.
+    + apply elem_of_cons; by right.
+    + by apply elem_of_cons in Hl2 as [Hcontr | Hl2]; [contradiction|].
+Qed.
+
+(* delete_list: delete a list of keys in a map *)
+
+Fixpoint delete_list {K V : Type} `{Countable K, EqDecision K}
+           (ks : list K) (m : gmap K V) : gmap K V :=
+  match ks with
+  | k :: ks' => delete k (delete_list ks' m)
+  | [] => m
+  end.
+
+Lemma delete_list_insert {K V : Type} `{Countable K, EqDecision K}
+      (ks : list K) (m : gmap K V) (l : K) (v : V) :
+  l ∉ ks →
+  delete_list ks (<[l:=v]> m) = <[l:=v]> (delete_list ks m).
+Proof.
+  intros Hnin.
+  induction ks; auto.
+  simpl.
+  apply not_elem_of_cons in Hnin as [Hneq Hnin].
+  rewrite -delete_insert_ne; auto.
+  f_equal. by apply IHks.
+Qed.
+
+Lemma delete_list_delete {K V : Type} `{Countable K, EqDecision K}
+      (ks : list K) (m : gmap K V) (l : K) :
+  l ∉ ks →
+  delete_list ks (delete l m) = delete l (delete_list ks m).
+Proof.
+  intros Hnin.
+  induction ks; auto.
+  simpl.
+  apply not_elem_of_cons in Hnin as [Hneq Hnin].
+  rewrite -delete_commute; auto.
+  f_equal. by apply IHks.
+Qed.
+
+Lemma lookup_delete_list_notin {K V : Type} `{Countable K, EqDecision K}
+      (ks : list K) (m : gmap K V) (l : K) :
+  l ∉ ks →
+  (delete_list ks m) !! l = m !! l.
+Proof.
+  intros HH; induction ks; simpl; auto.
+  eapply not_elem_of_cons in HH. destruct HH.
+  rewrite lookup_delete_ne; auto.
+Qed.
+
+Lemma delete_list_permutation {A B} `{Countable A, EqDecision A}
+      (l1 l2: list A) (m: gmap A B):
+  l1 ≡ₚ l2 → delete_list l1 m = delete_list l2 m.
+Proof.
+  induction 1.
+  { reflexivity. }
+  { cbn. rewrite IHPermutation //. }
+  { cbn. rewrite delete_commute //. }
+  { rewrite IHPermutation1 //. }
+Qed.
+
+Lemma delete_list_swap {A B : Type} `{EqDecision A, Countable A}
+      (a a' : A) (l1 l2 : list A) (M : gmap A B) :
+  delete a' (delete_list (l1 ++ a :: l2) M) =
+  delete a (delete a' (delete_list (l1 ++ l2) M)).
+Proof.
+  induction l1.
+  - apply delete_commute.
+  - simpl. repeat rewrite (delete_commute _ _ a0).
+    f_equiv. apply IHl1.
+Qed.
+
+(* Map difference for heterogeneous maps, and lemmas relating it to delete_list *)
+
+Definition map_difference_het
+  {A B C} `{Countable A, EqDecision A, Countable B, EqDecision B}
+  (m1: gmap A B) (m2: gmap A C): gmap A B
+:=
+  filter (fun '(k, v) => m2 !! k = None) m1.
+
+Notation "m1 ∖∖ m2" := (map_difference_het m1 m2) (at level 40, left associativity).
+
+Lemma map_eq' {A B} `{Countable A, EqDecision A, Countable B, EqDecision B}
+  (m1 m2: gmap A B):
+  m1 = m2 ↔ (forall k v, m1 !! k = Some v ↔ m2 !! k = Some v).
+Proof.
+  split. intros ->. done.
+  intros Heq. apply map_eq. intro k. destruct (m2 !! k) eqn:HH.
+  { by apply Heq. }
+  { destruct (m1 !! k) eqn:HHH; auto. apply Heq in HHH. congruence. }
+Qed.
+
+Lemma difference_het_lookup_Some
+    {A B C} `{Countable A, EqDecision A, Countable B, EqDecision B}
+    (m1: gmap A B) (m2: gmap A C) (k: A) (v: B):
+  (m1 ∖∖ m2) !! k = Some v ↔ m1 !! k = Some v ∧ m2 !! k = None.
+Proof. by rewrite /map_difference_het map_filter_lookup_Some. Qed.
+
+Lemma difference_het_lookup_None
+    {A B C} `{Countable A, EqDecision A, Countable B, EqDecision B}
+    (m1: gmap A B) (m2: gmap A C) (k: A) (v: B):
+  (m1 ∖∖ m2) !! k = None ↔ m1 !! k = None ∨ is_Some (m2 !! k).
+Proof.
+  rewrite /map_difference_het map_filter_lookup_None.
+  split; intros [HH1|HH2]; eauto.
+  { destruct (m1 !! k) eqn:?; eauto; right.
+    destruct (m2 !! k) eqn:?; eauto. exfalso. eapply HH2; eauto. }
+  { destruct (m1 !! k) eqn:?; eauto; right.
+    destruct (m2 !! k) eqn:?; eauto. destruct HH2 as [? ?]. congruence. }
+Qed.
+
+Lemma difference_het_empty
+  {A B C} `{Countable A, EqDecision A, Countable B, EqDecision B}
+  (m: gmap A B):
+  m ∖∖ (∅ : gmap A C) = m.
+Proof.
+  rewrite /map_difference_het map_eq'. intros k v.
+  rewrite map_filter_lookup_Some. rewrite lookup_empty. set_solver.
+Qed.
+
+ Lemma difference_het_eq_empty
+  {A B} `{Countable A, EqDecision A, Countable B, EqDecision B}
+  (m: gmap A B):
+  m ∖∖ m = (∅ : gmap A B).
+Proof.
+  rewrite /map_difference_het map_eq'. intros k v.
+  rewrite map_filter_lookup_Some. rewrite lookup_empty. set_solver.
+Qed.
+
+Lemma difference_het_insert_r
+    {A B C} `{Countable A, EqDecision A, Countable B, EqDecision B}
+    (m1: gmap A B) (m2: gmap A C) (k: A) (v: C):
+  m1 ∖∖ (<[ k := v ]> m2) = delete k (m1 ∖∖ m2).
+Proof.
+  intros.
+  rewrite /map_difference_het map_eq'. intros k' v'.
+  rewrite map_filter_lookup_Some lookup_delete_Some.
+  rewrite map_filter_lookup_Some lookup_insert_None. set_solver.
+Qed.
+
+Lemma difference_het_insert_l
+    {A B C} `{Countable A, EqDecision A, Countable B, EqDecision B}
+    (m1: gmap A B) (m2: gmap A C) (k: A) (v: B):
+  m2 !! k = None ->
+  <[ k := v ]> m1 ∖∖ m2 = <[ k := v ]> (m1 ∖∖ m2).
+Proof.
+  intros.
+  rewrite /map_difference_het map_eq'. intros k' v'.
+  rewrite map_filter_lookup_Some lookup_insert_Some.
+  rewrite -map_filter_insert;auto.
+    by rewrite map_filter_lookup_Some lookup_insert_Some.
+Qed.
+
+Lemma difference_het_delete_assoc
+    {A B C} `{Countable A, EqDecision A, Countable B, EqDecision B}
+    (m1: gmap A B) (m2: gmap A C) (k: A):
+  delete k (m1 ∖∖ m2) = (delete k m1) ∖∖ m2.
+Proof.
+  intros.
+  rewrite /map_difference_het map_eq'. intros k' v'.
+  rewrite map_filter_lookup_Some.
+  rewrite -map_filter_delete;auto.
+  rewrite map_filter_lookup_Some. set_solver.
+Qed.
+
+Lemma dom_difference_het
+    {A B C} `{Countable A, EqDecision A, Countable B, EqDecision B}
+    (m1: gmap A B) (m2: gmap A C):
+  dom (gset A) (m1 ∖∖ m2) = dom (gset A) m1 ∖ dom (gset A) m2.
+Proof.
+  apply (anti_symm _).
+  { rewrite elem_of_subseteq. intro k.
+    rewrite -elem_of_gmap_dom. intros [v Hv].
+    rewrite difference_het_lookup_Some in Hv * => Hv.
+    destruct Hv as [? ?].
+    rewrite elem_of_difference -!elem_of_gmap_dom. split; eauto.
+    intros [? ?]. congruence. }
+  { rewrite elem_of_subseteq. intro k.
+    rewrite elem_of_difference -!elem_of_gmap_dom. intros [[v ?] Hcontra].
+    exists v. rewrite difference_het_lookup_Some. split; eauto.
+    destruct (m2 !! k) eqn:?; eauto. exfalso. apply Hcontra. eauto. }
+Qed.
+
+Lemma delete_elements_eq_difference_het
+    {A B C} `{Countable A, EqDecision A, Countable B, EqDecision B}
+    (m1: gmap A B) (m2: gmap A C):
+  delete_list (elements (dom (gset A) m2)) m1 = m1 ∖∖ m2.
+Proof.
+  set (l := elements (dom (gset A) m2)).
+  assert (l ≡ₚ elements (dom (gset A) m2)) as Hl by reflexivity.
+  clearbody l. revert l Hl. revert m1. pattern m2. revert m2.
+  apply map_ind.
+  - intros m1 l. rewrite dom_empty_L elements_empty difference_het_empty.
+    rewrite Permutation_nil. intros ->. reflexivity.
+  - intros k v m2 Hm2k HI m1 l Hm1l.
+    rewrite difference_het_insert_r.
+    rewrite dom_insert in Hm1l * => Hm1l.
+    move: Hm1l. rewrite elements_union_singleton.
+    2: rewrite -elem_of_gmap_dom; intros [? ?]; congruence.
+    intros Hm1l.
+    transitivity (delete k (delete_list (elements (dom (gset A) m2)) m1)).
+    { erewrite delete_list_permutation. 2: eauto. reflexivity. }
+    { rewrite HI//. }
+Qed.
+
+(* rtc *)
+
+Lemma rtc_implies {A : Type} (R Q : A → A → Prop) (x y : A) :
+  (∀ r q, R r q → Q r q) →
+  rtc R x y → rtc Q x y.
+Proof.
+  intros Himpl HR.
+  induction HR.
+  - done.
+  - apply Himpl in H.
+    apply rtc_once in H.
+    apply rtc_transitive with y; auto.
+Qed.
+
+Lemma rtc_or_intro {A : Type} (R Q : A → A → Prop) (x y : A) :
+  rtc (λ a b, R a b) x y →
+  rtc (λ a b, R a b ∨ Q a b) x y.
+Proof.
+  intros HR. induction HR.
+  - done.
+  - apply rtc_transitive with y; auto.
+    apply rtc_once. by left.
+Qed.
+
+Lemma rtc_or_intro_l {A : Type} (R Q : A → A → Prop) (x y : A) :
+    rtc (λ a b, R a b) x y →
+    rtc (λ a b, Q a b ∨ R a b) x y.
+Proof.
+  intros HR. induction HR.
+  - done.
+  - apply rtc_transitive with y; auto.
+    apply rtc_once. by right.
+Qed.
+
+ (* Helper lemmas on list differences *)
+
+Lemma not_elem_of_list {A : Type} `{EqDecision A} (a : A) (l x : list A) :
+  a ∈ x → a ∉ list_difference l x.
+Proof.
+  intros Hax.
+  rewrite /not.
+  intros Hal.
+  by apply elem_of_list_difference in Hal as [Ha' Hax_not].
+Qed.
+
+Lemma list_difference_nil {A : Type} `{EqDecision A} (l : list A) :
+  list_difference l [] = l.
+Proof.
+  induction l; auto.
+  simpl. f_equal.
+  apply IHl.
+Qed.
+
+Lemma list_difference_length_cons {A : Type} `{EqDecision A}
+      (l2 : list A) (a : A) :
+  list_difference [a] (a :: l2) = [].
+Proof.
+  simpl.
+  assert (a ∈ a :: l2); first apply elem_of_list_here.
+  destruct (decide_rel elem_of a (a :: l2)); auto; last contradiction.
+Qed.
+
+Lemma list_difference_skip {A : Type} `{EqDecision A}
+      (l1 l2 : list A) (b : A) :
+  ¬ (b ∈ l1) →
+  list_difference l1 (b :: l2) = list_difference l1 l2.
+Proof.
+  intros Hnin.
+  induction l1; auto.
+  apply not_elem_of_cons in Hnin.
+  destruct Hnin as [Hne Hl1].
+  simpl.
+  destruct (decide_rel elem_of a (b :: l2)).
+  - apply elem_of_cons in e.
+    destruct e as [Hcontr | Hl2]; first congruence.
+    destruct (decide_rel elem_of a l2); last contradiction.
+      by apply IHl1.
+  - apply not_elem_of_cons in n.
+    destruct n as [Hne' Hl2].
+    destruct (decide_rel elem_of a l2); first contradiction.
+    f_equal.
+      by apply IHl1.
+Qed.
+
+Lemma list_difference_nested {A : Type} `{EqDecision A}
+      (l1 l1' l2 : list A) (b : A) :
+  ¬ (b ∈ (l1 ++ l1')) →
+  list_difference (l1 ++ b :: l1') (b :: l2) = list_difference (l1 ++ l1') l2.
+Proof.
+  intros Hnotin.
+  induction l1.
+  - simpl.
+    assert (b ∈ (b :: l2)); first apply elem_of_list_here.
+    destruct (decide_rel elem_of b (b :: l2)); last contradiction.
+    rewrite list_difference_skip; auto.
+  - simpl in *.
+    apply not_elem_of_cons in Hnotin.
+    destruct Hnotin as [Hne Hnotin].
+    destruct (decide_rel elem_of a (b :: l2)).
+    + apply elem_of_cons in e.
+      destruct e as [Hcontr | Hl2]; first congruence.
+      destruct (decide_rel elem_of a l2); last contradiction.
+        by apply IHl1.
+    + apply not_elem_of_cons in n.
+      destruct n as [Hne' Hnotin'].
+      destruct (decide_rel elem_of a l2); first contradiction.
+      f_equal.
+        by apply IHl1.
+Qed.
+
+Lemma list_difference_length_ni  {A : Type} `{EqDecision A}
+      (l1 : list A) (b : A) :
+  ¬ (b ∈ l1) →
+  length (list_difference l1 [b]) = length l1.
+Proof.
+  intros Hna.
+  destruct l1; auto.
+  simpl.
+  apply not_elem_of_cons in Hna.
+  destruct Hna as [Hne Hna].
+  destruct (decide_rel elem_of a [b]).
+  - apply elem_of_list_singleton in e. congruence.
+  - simpl. rewrite list_difference_skip; auto.
+      by rewrite list_difference_nil.
+Qed.
+
+Lemma list_difference_length {A : Type} `{EqDecision A}
+      (l1 : list A) (b : A) :
+  b ∈ l1 →
+  NoDup l1 →
+  length (list_difference l1 [b]) =
+  length l1 - 1.
+Proof.
+  intros Ha Hndup.
+  induction l1; auto.
+  destruct (decide (b = a)).
+  - subst.
+    assert (a ∈ a :: l1); first apply elem_of_list_here.
+    rewrite ->NoDup_cons in Hndup. destruct Hndup as [Hni Hndup].
+    assert (¬ (a ∈ l1)) as Hni'.
+    { rewrite /not. intros Hin. contradiction. }
+    simpl.
+    assert (a ∈ [a]); first apply elem_of_list_here.
+    destruct (decide_rel elem_of a [a]); last contradiction.
+    rewrite -minus_n_O.
+    apply list_difference_length_ni; auto.
+  - simpl.
+    assert (¬ (a ∈ [b])).
+    { rewrite /not. intros Hin. apply elem_of_list_singleton in Hin. congruence. }
+    destruct (decide_rel elem_of a [b]); first contradiction.
+    rewrite -minus_n_O /=.
+    inversion Hndup; subst.
+    apply elem_of_cons in Ha.
+    destruct Ha as [Hcontr | Ha]; first congruence.
+    apply IHl1 in Ha as Heq; auto.
+    rewrite Heq.
+    destruct l1; first inversion Ha.
+    simpl. lia.
+Qed.
+
+Lemma list_difference_app {A : Type} `{EqDecision A}
+      (l1 l2 l2' : list A) :
+  list_difference l1 (l2 ++ l2') = list_difference (list_difference l1 l2) l2'.
+Proof.
+  induction l1; auto.
+  simpl. destruct (decide_rel elem_of a (l2 ++ l2')).
+  - apply elem_of_app in e as [Hl2 | Hl2'].
+    + destruct (decide_rel elem_of a l2); last contradiction.
+      apply IHl1.
+    + destruct (decide_rel elem_of a l2); first by apply IHl1.
+      simpl.
+      destruct (decide_rel elem_of a l2'); last contradiction.
+      apply IHl1.
+  - apply not_elem_of_app in n as [Hl2 Hl2'].
+    destruct (decide_rel elem_of a l2); first contradiction.
+    simpl.
+    destruct (decide_rel elem_of a l2'); first contradiction.
+    f_equal. apply IHl1.
+Qed.
+
+Lemma list_difference_Permutation {A : Type} `{EqDecision A} (l l1 l2 : list A) :
+  l1 ≡ₚ l2 -> list_difference l l1 = list_difference l l2.
+Proof.
+  intros Hl.
+  induction l; auto.
+  simpl. rewrite IHl.
+  destruct (decide_rel elem_of a l1).
+  - apply elem_of_list_In in e.
+    apply Permutation_in with _ _ _ a in Hl; auto.
+    apply elem_of_list_In in Hl.
+    destruct (decide_rel elem_of a l2);[|contradiction].
+    done.
+  - revert n; rewrite elem_of_list_In; intros n.
+    assert (¬ In a l2) as Hnin.
+    { intros Hcontr. apply Permutation_sym in Hl.
+      apply Permutation_in with _ _ _ a in Hl; auto. }
+    revert Hnin; rewrite -elem_of_list_In; intro Hnin.
+    destruct (decide_rel elem_of a l2);[contradiction|].
+    done.
+Qed.
+
+Lemma list_to_set_difference A {_: EqDecision A} {_: Countable A} (l1 l2: list A):
+  (list_to_set (list_difference l1 l2): gset A) = (list_to_set l1: gset A) ∖ (list_to_set l2: gset A).
+Proof.
+  revert l2. induction l1.
+  - intro. cbn [list_difference list_to_set]. set_solver.
+  - intros l2. cbn [list_difference list_to_set]. destruct (decide_rel elem_of a l2); set_solver.
+Qed.
+
+(* creates a gmap with domain from the list, all pointing to a default value *)
+Fixpoint create_gmap_default {K V : Type} `{Countable K}
+         (l : list K) (d : V) : gmap K V :=
+  match l with
+  | [] => ∅
+  | k :: tl => <[k:=d]> (create_gmap_default tl d)
+  end.
+
+Lemma create_gmap_default_lookup {K V : Type} `{Countable K}
+      (l : list K) (d : V) (k : K) :
+  k ∈ l ↔ (create_gmap_default l d) !! k = Some d.
+Proof.
+  split.
+  - intros Hk.
+    induction l; inversion Hk.
+    + by rewrite lookup_insert.
+    + destruct (decide (a = k)); [subst; by rewrite lookup_insert|].
+      rewrite lookup_insert_ne; auto.
+  - intros Hl.
+    induction l; inversion Hl.
+    destruct (decide (a = k)); [subst;apply elem_of_list_here|].
+    apply elem_of_cons. right.
+    apply IHl. simplify_map_eq. auto.
+Qed.
+
+Lemma create_gmap_default_lookup_is_Some {K V} `{EqDecision K, Countable K} (l: list K) (d: V) x v:
+  create_gmap_default l d !! x = Some v → x ∈ l ∧ v = d.
+Proof.
+  revert x v d. induction l as [| a l]; cbn.
+  - done.
+  - intros x v d. destruct (decide (a = x)) as [->|].
+    + rewrite lookup_insert. intros; simplify_eq. repeat constructor.
+    + rewrite lookup_insert_ne //. intros [? ?]%IHl. subst. repeat constructor; auto.
+Qed.
+
+Lemma create_gmap_default_dom {K V} `{EqDecision K, Countable K} (l: list K) (d: V):
+  dom (gset K) (create_gmap_default l d) = list_to_set l.
+Proof.
+  induction l as [| a l].
+  - cbn. rewrite dom_empty_L //.
+  - cbn [create_gmap_default list_to_set]. rewrite dom_insert_L // IHl //.
+Qed.
+
