theories/examples/stack_macros_helpers.v
@@ -7,50 +7,6 @@ From cap_machine Require Import cap_lang region contiguous.
 Section helpers.
 
   (* ---------------------------- Helper Lemmas --------------------------------------- *)
-  (* TODO: move to lang *)
-  Lemma isCorrectPC_bounds_alt p g b e (a0 a1 a2 : Addr) :
-    isCorrectPC (inr (p, g, b, e, a0))
-    → isCorrectPC (inr (p, g, b, e, a2))
-    → (a0 ≤ a1)%Z ∧ (a1 ≤ a2)%Z
-    → isCorrectPC (inr (p, g, b, e, a1)).
-  Proof.
-    intros Hvpc0 Hvpc2 [Hle0 Hle2].
-    apply Z.lt_eq_cases in Hle2 as [Hlt2 | Heq2].
-    - apply isCorrectPC_bounds with a0 a2; auto.
-    - apply z_of_eq in Heq2. rewrite Heq2. auto.
-  Qed.
-
-  Lemma isWithinBounds_bounds_alt p g b e (a0 a1 a2 : Addr) :
-    withinBounds (p,g,b,e,a0) = true ->
-    withinBounds (p,g,b,e,a2) = true ->
-    (a0 ≤ a1)%Z ∧ (a1 ≤ a2)%Z ->
-    withinBounds (p,g,b,e,a1) = true.
-  Proof.
-    intros Hwb0 Hwb2 [Hle0 Hle2].
-    rewrite /withinBounds.
-    apply andb_true_iff.
-    apply andb_true_iff in Hwb0 as [Hleb0 Hlea0].
-    apply andb_true_iff in Hwb2 as [Hleb2 Hlea2].
-    split; rewrite /leb_addr /ltb_addr; first [ apply Z.leb_le | apply Z.ltb_lt ].
-    - apply Z.leb_le in Hleb0. apply Z.ltb_lt in Hlea0. lia.
-    - apply Z.leb_le in Hleb2. apply Z.ltb_lt in Hlea2. lia.
-  Qed.
-
-  Lemma isWithinBounds_bounds_alt' p g b e (a0 a1 a2 : Addr) :
-    withinBounds (p,g,b,e,a0) = true ->
-    withinBounds (p,g,b,e,a2) = true ->
-    (a0 ≤ a1)%Z ∧ (a1 < a2)%Z ->
-    withinBounds (p,g,b,e,a1) = true.
-  Proof.
-    intros Hwb0 Hwb2 [Hle0 Hle2].
-    rewrite /withinBounds.
-    apply andb_true_iff.
-    apply andb_true_iff in Hwb0 as [Hleb0 Hlea0].
-    apply andb_true_iff in Hwb2 as [Hleb2 Hlea2].
-    split; rewrite /leb_addr /ltb_addr; first [ apply Z.leb_le | apply Z.ltb_lt ].
-    - apply Z.leb_le in Hleb0. apply Z.ltb_lt in Hlea0. lia.
-    - apply Z.leb_le in Hleb2. apply Z.ltb_lt in Hlea2. lia.
-  Qed.
 
   Definition isCorrectPC_range p g b e a0 an :=
     ∀ ai, (a0 <= ai)%a ∧ (ai < an)%a → isCorrectPC (inr (p, g, b, e, ai)).
@@ -84,31 +40,14 @@ Section helpers.
     inversion HH; auto.
   Qed.
 
-  
-
-  Lemma delete_eq {A : Type} (a : list A) i :
-    strings.length a ≤ i -> a = delete i a.
+  Lemma isCorrectPC_range_npE p g b e a0 an :
+    isCorrectPC_range p g b e a0 an →
+    (a0 < an)%a →
+    p ≠ E.
   Proof.
-    revert i. induction a; intros i Hle.
-    - done.
-    - destruct i; [inversion Hle|].
-      simpl. f_equiv. apply IHa. simpl in Hle. lia.
-  Qed. 
-  
-  Lemma delete_insert_list {A : Type} i (l : list A) (a : A) :
-    <[i := a]> (delete 0 l) = delete 0 (<[S i := a]> l).
-  Proof.
-    induction l.
-    - done.
-    - simpl in *. destruct l; auto. 
+    intros HH1 HH2.
+    destruct (isCorrectPC_range_perm _ _ _ _ _ _ HH1 HH2) as [?| [?|?] ];
+      congruence.
   Qed.
 
-  Lemma insert_delete_list {A : Type} (l : list A) (a : A) :
-    delete 0 (<[0 := a]> l) = delete 0 l.
-  Proof.
-    induction l; done.
-  Qed. 
-
-End helpers. 
-
-  
+End helpers.
