theories/iris_extra.v
@@ -1,6 +1,7 @@
 From iris.algebra Require Import frac.
 From iris.proofmode Require Import tactics.
 From iris.base_logic Require Import invariants.
+From cap_machine Require Import stdpp_extra.
 
 Lemma big_sepM_to_big_sepL {Σ : gFunctors} {A B : Type} `{EqDecision A} `{Countable A}
       (r : gmap A B) (lr : list A) (φ : A → B → iProp Σ) :
@@ -72,105 +73,95 @@ Proof.
   rewrite delete_take_drop. iFrame.
 Qed.
 
-Lemma drop_S:
-    forall A l n (a: A) l',
-      drop n l = a::l' ->
-      drop (S n) l = l'.
-  Proof.
-    induction l; intros * HH.
-    - rewrite drop_nil in HH. inversion HH.
-    - simpl. destruct n.
-      + rewrite drop_0 in HH. inversion HH.
-        reflexivity.
-      + simpl in HH. eapply IHl; eauto.
-  Qed.
-
 Lemma big_sepL2_extract_l' {Σ : gFunctors} {A B : Type} (i : nat) (ai : A) (a : list A) (b : list B) (φ : A -> B -> iProp Σ) :
     a !! i = Some ai ->
     (([∗ list] a_i;b_i ∈ a;b, φ a_i b_i) -∗
      ([∗ list] a_i;b_i ∈ (delete i a);(delete i b), φ a_i b_i) ∗ ∃ b, φ ai b)%I.
-  Proof. 
-    iIntros (Hsome) "Hl".
-    iDestruct (big_sepL2_length with "Hl") as %Hlength.      
-    assert (take i a ++ drop i a = a) as Heqa;[apply take_drop|]. 
-    assert (take i b ++ drop i b = b) as Heqb;[apply take_drop|]. 
-    rewrite -Heqa -Heqb.
-    iDestruct (big_sepL2_app_inv with "Hl") as "[Htake Hdrop]". 
-    { apply lookup_lt_Some in Hsome.
-      do 2 (rewrite take_length_le;[|lia]). done. 
-    }
-    apply take_drop_middle in Hsome as Hcons.
-    assert (ai :: drop (S i) a = drop i a) as Hh.
-    { apply app_inv_head with (take i a). congruence. }
-    rewrite -Hh.
-    iDestruct (big_sepL2_length with "Hdrop") as %Hlength'.      
-    destruct (drop i b);[inversion Hlength'|].
-    iDestruct "Hdrop" as "[Hφ Hdrop]".
-    iSplitR "Hφ";[|eauto].
-    rewrite Hcons. iDestruct (big_sepL2_app with "Htake Hdrop") as "Hl".
-    rewrite Heqb. rewrite (delete_take_drop a).
-    rewrite (delete_take_drop b).
-    assert (drop (S i) b = l) as Hb.
-    { apply app_inv_head with (take i b ++ [b0]). repeat rewrite -app_assoc.
-      repeat rewrite -cons_middle. rewrite (drop_S _ _ _ b0 l);auto.
-      apply app_inv_head with (take i b). rewrite Heqb. apply take_drop. }
-    rewrite Hb. iFrame. 
-  Qed.
+Proof.
+  iIntros (Hsome) "Hl".
+  iDestruct (big_sepL2_length with "Hl") as %Hlength.
+  assert (take i a ++ drop i a = a) as Heqa;[apply take_drop|].
+  assert (take i b ++ drop i b = b) as Heqb;[apply take_drop|].
+  rewrite -Heqa -Heqb.
+  iDestruct (big_sepL2_app_inv with "Hl") as "[Htake Hdrop]".
+  { apply lookup_lt_Some in Hsome.
+    do 2 (rewrite take_length_le;[|lia]). done.
+  }
+  apply take_drop_middle in Hsome as Hcons.
+  assert (ai :: drop (S i) a = drop i a) as Hh.
+  { apply app_inv_head with (take i a). congruence. }
+  rewrite -Hh.
+  iDestruct (big_sepL2_length with "Hdrop") as %Hlength'.
+  destruct (drop i b);[inversion Hlength'|].
+  iDestruct "Hdrop" as "[Hφ Hdrop]".
+  iSplitR "Hφ";[|eauto].
+  rewrite Hcons. iDestruct (big_sepL2_app with "Htake Hdrop") as "Hl".
+  rewrite Heqb. rewrite (delete_take_drop a).
+  rewrite (delete_take_drop b).
+  assert (drop (S i) b = l) as Hb.
+  { pose proof (take_drop_middle b i b0) as HH.
+    enough (b0 :: drop (S i) b = b0 :: l) as He by (inversion He; auto).
+    eapply (app_inv_head (take i b)). rewrite HH //.
+    rewrite -Heqb. apply list_lookup_middle.
+    rewrite take_length_le //. enough (i < length b) by lia.
+    rewrite -Hlength. apply lookup_lt_is_Some. eauto. }
+  rewrite Hb. iFrame.
+Qed.
 
-  Lemma big_sepL2_extract' {Σ : gFunctors} {A B : Type} (i : nat) (ai : A) (bi : B) (a : list A) (b : list B) (φ : A -> B -> iProp Σ) :
-    a !! i = Some ai -> b !! i = Some bi ->
-    (([∗ list] a_i;b_i ∈ a;b, φ a_i b_i) -∗
-     ([∗ list] a_i;b_i ∈ (delete i a);(delete i b), φ a_i b_i) ∗ φ ai bi)%I.
-  Proof. 
-    iIntros (Hsome Hsome') "Hl".
-    iDestruct (big_sepL2_length with "Hl") as %Hlength.      
-    assert (take i a ++ drop i a = a) as Heqa;[apply take_drop|]. 
-    assert (take i b ++ drop i b = b) as Heqb;[apply take_drop|]. 
-    rewrite -Heqa -Heqb.
-    iDestruct (big_sepL2_app_inv with "Hl") as "[Htake Hdrop]". 
-    { apply lookup_lt_Some in Hsome.
-      do 2 (rewrite take_length_le;[|lia]). done. 
-    }
-    apply take_drop_middle in Hsome as Hcons.
-    apply take_drop_middle in Hsome' as Hcons'.
-    assert (ai :: drop (S i) a = drop i a) as Hh.
-    { apply app_inv_head with (take i a). congruence. }
-    assert (bi :: drop (S i) b = drop i b) as Hhb.
-    { apply app_inv_head with (take i b). congruence. }
-    rewrite -Hh. rewrite -Hhb.
-    iDestruct "Hdrop" as "[Hφ Hdrop]".
-    iSplitR "Hφ";[|eauto].
-    rewrite Hcons. rewrite Hcons'. iDestruct (big_sepL2_app with "Htake Hdrop") as "Hl".
-    rewrite (delete_take_drop b). rewrite (delete_take_drop a). iFrame. 
-  Qed.
+Lemma big_sepL2_extract' {Σ : gFunctors} {A B : Type} (i : nat) (ai : A) (bi : B) (a : list A) (b : list B) (φ : A -> B -> iProp Σ) :
+  a !! i = Some ai -> b !! i = Some bi ->
+  (([∗ list] a_i;b_i ∈ a;b, φ a_i b_i) -∗
+   ([∗ list] a_i;b_i ∈ (delete i a);(delete i b), φ a_i b_i) ∗ φ ai bi)%I.
+Proof.
+  iIntros (Hsome Hsome') "Hl".
+  iDestruct (big_sepL2_length with "Hl") as %Hlength.
+  assert (take i a ++ drop i a = a) as Heqa;[apply take_drop|].
+  assert (take i b ++ drop i b = b) as Heqb;[apply take_drop|].
+  rewrite -Heqa -Heqb.
+  iDestruct (big_sepL2_app_inv with "Hl") as "[Htake Hdrop]".
+  { apply lookup_lt_Some in Hsome.
+    do 2 (rewrite take_length_le;[|lia]). done.
+  }
+  apply take_drop_middle in Hsome as Hcons.
+  apply take_drop_middle in Hsome' as Hcons'.
+  assert (ai :: drop (S i) a = drop i a) as Hh.
+  { apply app_inv_head with (take i a). congruence. }
+  assert (bi :: drop (S i) b = drop i b) as Hhb.
+  { apply app_inv_head with (take i b). congruence. }
+  rewrite -Hh. rewrite -Hhb.
+  iDestruct "Hdrop" as "[Hφ Hdrop]".
+  iSplitR "Hφ";[|eauto].
+  rewrite Hcons. rewrite Hcons'. iDestruct (big_sepL2_app with "Htake Hdrop") as "Hl".
+  rewrite (delete_take_drop b). rewrite (delete_take_drop a). iFrame.
+Qed.
 
-  Lemma big_sepL2_close_l {Σ : gFunctors} {A B : Type} (i : nat) (ai : A) (bi : B) (a : list A) (b : list B) (φ : A -> B -> iProp Σ) :
-    length a = length b ->
-    a !! i = Some ai ->
-    (([∗ list] a_i;b_i ∈ (delete i a);(delete i b), φ a_i b_i) ∗ φ ai bi -∗
-                                                               ([∗ list] a_i;b_i ∈ a;<[i:= bi]> b, φ a_i b_i) )%I.
-  Proof. 
-    iIntros (Hlen Hsome) "[Hl Hb]".
-    iDestruct (big_sepL2_length with "Hl") as %Hlength.
-    repeat rewrite delete_take_drop.
-    apply lookup_lt_Some in Hsome as Hlt.
-    assert (i < strings.length b) as Hlt';[lia|].
-    iDestruct (big_sepL2_app_inv with "Hl") as "[Htake Hdrop]". 
-    { repeat rewrite take_length. lia. }
-    apply take_drop_middle in Hsome as Hcons.
-    assert (ai :: drop (S i) a = drop i a) as Hh.
-    { apply app_inv_head with (take i a). rewrite Hcons. by rewrite take_drop. }
-    iAssert ([∗ list] y1;y2 ∈ ai :: drop (S i) a;bi :: drop (S i) b, φ y1 y2)%I
-      with "[Hb Hdrop]" as "Hdrop";[iFrame|].
-    rewrite Hh.
-    iDestruct (big_sepL2_app with "Htake Hdrop") as "Hab".
-    rewrite take_drop.
-    assert (take i b ++ bi :: drop (S i) b = <[i:=bi]> b) as ->;[|iFrame].
-    assert (<[i:=bi]> b !! i = Some bi) as Hsome'.
-    { apply list_lookup_insert. lia. }
-    apply take_drop_middle in Hsome'. rewrite -Hsome'.
-    rewrite take_insert;[|lia]. rewrite drop_insert;[|lia]. done. 
-  Qed.
+Lemma big_sepL2_close_l {Σ : gFunctors} {A B : Type} (i : nat) (ai : A) (bi : B) (a : list A) (b : list B) (φ : A -> B -> iProp Σ) :
+  length a = length b ->
+  a !! i = Some ai ->
+  (([∗ list] a_i;b_i ∈ (delete i a);(delete i b), φ a_i b_i) ∗ φ ai bi -∗
+                                                             ([∗ list] a_i;b_i ∈ a;<[i:= bi]> b, φ a_i b_i) )%I.
+Proof.
+  iIntros (Hlen Hsome) "[Hl Hb]".
+  iDestruct (big_sepL2_length with "Hl") as %Hlength.
+  repeat rewrite delete_take_drop.
+  apply lookup_lt_Some in Hsome as Hlt.
+  assert (i < strings.length b) as Hlt';[lia|].
+  iDestruct (big_sepL2_app_inv with "Hl") as "[Htake Hdrop]".
+  { repeat rewrite take_length. lia. }
+  apply take_drop_middle in Hsome as Hcons.
+  assert (ai :: drop (S i) a = drop i a) as Hh.
+  { apply app_inv_head with (take i a). rewrite Hcons. by rewrite take_drop. }
+  iAssert ([∗ list] y1;y2 ∈ ai :: drop (S i) a;bi :: drop (S i) b, φ y1 y2)%I
+    with "[Hb Hdrop]" as "Hdrop";[iFrame|].
+  rewrite Hh.
+  iDestruct (big_sepL2_app with "Htake Hdrop") as "Hab".
+  rewrite take_drop.
+  assert (take i b ++ bi :: drop (S i) b = <[i:=bi]> b) as ->;[|iFrame].
+  assert (<[i:=bi]> b !! i = Some bi) as Hsome'.
+  { apply list_lookup_insert. lia. }
+  apply take_drop_middle in Hsome'. rewrite -Hsome'.
+  rewrite take_insert;[|lia]. rewrite drop_insert;[|lia]. done.
+Qed.
 
 Lemma region_addrs_exists `{Σ : gFunctors} {A B: Type} (a : list A) (φ : A → B → iProp Σ) :
      (([∗ list] a0 ∈ a, (∃ b0, φ a0 b0)) ∗-∗
@@ -196,7 +187,7 @@ Qed.
 
 Lemma region_addrs_exists_zip `{Σ : gFunctors} {A B C: Type} (a : list A) (φ : A → B → C -> iProp Σ) :
   (([∗ list] a0 ∈ a, (∃ b0 c0, φ a0 b0 c0)) ∗-∗
-                                            (∃ (ws : list (B * C)), [∗ list] a0;bc0 ∈ a;ws, φ a0 bc0.1 bc0.2))%I.
+  (∃ (ws : list (B * C)), [∗ list] a0;bc0 ∈ a;ws, φ a0 bc0.1 bc0.2))%I.
 Proof.
   iSplit. 
   - iIntros "Ha".
@@ -264,155 +255,185 @@ Proof.
       iFrame. iApply "Hl2". auto. 
 Qed.
 
-   Lemma big_sepL2_to_big_sepL_l `{Σ : gFunctors} {A B : Type} (φ : A → iProp Σ) (l1 : list A)
-         (l2 : list B) :
-     length l1 = length l2 →
-     (([∗ list] y1;_ ∈ l1;l2, φ y1) ∗-∗
-     ([∗ list] y ∈ l1, φ y))%I. 
-   Proof.
-     iIntros (Hlen). 
-     iSplit. 
-     - iIntros "Hl2". iRevert (Hlen). 
-       iInduction (l1) as [ | y1] "IHn" forall (l2); iIntros (Hlen). 
-       + done.
-       + destruct l2;[by iApply bi.False_elim|]. 
-         iDestruct "Hl2" as "[$ Hl2]". 
-         iApply ("IHn" with "Hl2"). auto. 
-     - iIntros "Hl2". 
-       iRevert (Hlen). 
-       iInduction (l1) as [ | y1] "IHn" forall (l2); iIntros (Hlen). 
-       + destruct l2; inversion Hlen. done.
-       + iDestruct "Hl2" as "[Hy2 Hl2]".
-         destruct l2; inversion Hlen. 
-         iDestruct ("IHn" $! l2 with "Hl2") as "Hl2".
-         iFrame. iApply "Hl2". auto. 
-   Qed.
+Lemma big_sepL2_to_big_sepL_l `{Σ : gFunctors} {A B : Type} (φ : A → iProp Σ) (l1 : list A)
+      (l2 : list B) :
+  length l1 = length l2 →
+  (([∗ list] y1;_ ∈ l1;l2, φ y1) ∗-∗
+  ([∗ list] y ∈ l1, φ y))%I.
+Proof.
+  iIntros (Hlen).
+  iSplit.
+  - iIntros "Hl2". iRevert (Hlen).
+    iInduction (l1) as [ | y1] "IHn" forall (l2); iIntros (Hlen).
+    + done.
+    + destruct l2;[by iApply bi.False_elim|].
+      iDestruct "Hl2" as "[$ Hl2]".
+      iApply ("IHn" with "Hl2"). auto.
+  - iIntros "Hl2".
+    iRevert (Hlen).
+    iInduction (l1) as [ | y1] "IHn" forall (l2); iIntros (Hlen).
+    + destruct l2; inversion Hlen. done.
+    + iDestruct "Hl2" as "[Hy2 Hl2]".
+      destruct l2; inversion Hlen.
+      iDestruct ("IHn" $! l2 with "Hl2") as "Hl2".
+      iFrame. iApply "Hl2". auto.
+Qed.
 
-   Lemma big_sepL2_app'
-         (PROP : bi) (A B : Type) (Φ : nat → A → B → PROP) (l1 l2 : list A)
-         (l1' l2' : list B) :
-     (length l1) = (length l1') →
-     (([∗ list] k↦y1;y2 ∈ l1;l1', Φ k y1 y2)
-        ∗ ([∗ list] k↦y1;y2 ∈ l2;l2', Φ (strings.length l1 + k) y1 y2))%I
-      ≡ ([∗ list] k↦y1;y2 ∈ (l1 ++ l2);(l1' ++ l2'), Φ k y1 y2)%I.
-   Proof.
-     intros Hlenl1.
-     iSplit.
-     - iIntros "[Hl1 Hl2]". iApply (big_sepL2_app with "Hl1 Hl2").
-     - iIntros "Happ".
-       iAssert (∃ l0' l0'' : list A,
-                   ⌜(l1 ++ l2) = l0' ++ l0''⌝
-                   ∧ ([∗ list] k↦y1;y2 ∈ l0';l1', Φ k y1 y2)
-                       ∗ ([∗ list] k↦y1;y2 ∈ l0'';l2', Φ (strings.length l1' + k) y1 y2))%I
-         with "[Happ]" as (l0' l0'') "(% & Happl0' & Happl0'')".
-       { by iApply (big_sepL2_app_inv_r with "Happ"). }
-       iDestruct (big_sepL2_length with "Happl0'") as %Hlen1.
-       iDestruct (big_sepL2_length with "Happl0''") as %Hlen2.
-       rewrite -Hlenl1 in Hlen1.
-       assert (l1 = l0' ∧ l2 = l0'') as [Heq1 Heq2]; first by apply app_inj_1.
-       simplify_eq; rewrite Hlenl1.
-       iFrame.
-   Qed.
-
-   Lemma big_sepL2_split_at `{Σ : gFunctors} {A B: Type} `{EqDecision A} `{Countable A}
-        (k: nat) (l1: list A) (l2: list B) (φ : A → B → iProp Σ):
-    ([∗ list] a;b ∈ l1;l2, φ a b) -∗
-    ([∗ list] a;b ∈ (take k l1);(take k l2), φ a b) ∗ ([∗ list] a;b ∈ (drop k l1);(drop k l2), φ a b).
-  Proof.
-    iIntros "H".
-    iDestruct (big_sepL2_length with "H") as %?.
-    rewrite -{1}(take_drop k l1) -{1}(take_drop k l2).
-    iDestruct (big_sepL2_app' with "H") as "[? ?]".
-    { rewrite !take_length. lia. }
+Lemma big_sepL2_app'
+      (PROP : bi) (A B : Type) (Φ : nat → A → B → PROP) (l1 l2 : list A)
+      (l1' l2' : list B) :
+  (length l1) = (length l1') →
+  (([∗ list] k↦y1;y2 ∈ l1;l1', Φ k y1 y2)
+     ∗ ([∗ list] k↦y1;y2 ∈ l2;l2', Φ (strings.length l1 + k) y1 y2))%I
+   ≡ ([∗ list] k↦y1;y2 ∈ (l1 ++ l2);(l1' ++ l2'), Φ k y1 y2)%I.
+Proof.
+  intros Hlenl1.
+  iSplit.
+  - iIntros "[Hl1 Hl2]". iApply (big_sepL2_app with "Hl1 Hl2").
+  - iIntros "Happ".
+    iAssert (∃ l0' l0'' : list A,
+                ⌜(l1 ++ l2) = l0' ++ l0''⌝
+                ∧ ([∗ list] k↦y1;y2 ∈ l0';l1', Φ k y1 y2)
+                    ∗ ([∗ list] k↦y1;y2 ∈ l0'';l2', Φ (strings.length l1' + k) y1 y2))%I
+      with "[Happ]" as (l0' l0'') "(% & Happl0' & Happl0'')".
+    { by iApply (big_sepL2_app_inv_r with "Happ"). }
+    iDestruct (big_sepL2_length with "Happl0'") as %Hlen1.
+    iDestruct (big_sepL2_length with "Happl0''") as %Hlen2.
+    rewrite -Hlenl1 in Hlen1.
+    assert (l1 = l0' ∧ l2 = l0'') as [Heq1 Heq2]; first by apply app_inj_1.
+    simplify_eq; rewrite Hlenl1.
     iFrame.
-  Qed.
+Qed.
 
-  Lemma big_sepL_delete' {PROP: bi} {A: Type} (φ: A -> PROP) (l: list A):
-        forall k, (([∗ list] k0↦y ∈ l, if decide (k0 = k) then emp else φ y) -∗
-             ([∗ list] k0↦x0 ∈ delete k l, (λ (_ : nat) (x1 : A), φ x1) k0 x0))%I.
-  Proof.
-    iInduction (l) as [|x l] "IH"; simpl; auto; iIntros (k) "H".
-    iDestruct "H" as "[H1 H2]".
-    rewrite /delete /=. destruct k.
-    - iApply (big_sepL_impl with "H2").
-      iClear "H1". iModIntro. iIntros. destruct (decide (S k = 0)); auto. lia.
-    - simpl. iFrame. iApply ("IH" with "[H2]").
-      iApply (big_sepL_impl with "H2").
-      iModIntro; iIntros. destruct (decide (k0 = k)); destruct (decide (S k0 = S k)); auto; lia.
-  Qed.
+Lemma big_sepL2_split_at `{Σ : gFunctors} {A B: Type} `{EqDecision A} `{Countable A}
+      (k: nat) (l1: list A) (l2: list B) (φ : A → B → iProp Σ):
+  ([∗ list] a;b ∈ l1;l2, φ a b) -∗
+  ([∗ list] a;b ∈ (take k l1);(take k l2), φ a b) ∗ ([∗ list] a;b ∈ (drop k l1);(drop k l2), φ a b).
+Proof.
+  iIntros "H".
+  iDestruct (big_sepL2_length with "H") as %?.
+  rewrite -{1}(take_drop k l1) -{1}(take_drop k l2).
+  iDestruct (big_sepL2_app' with "H") as "[? ?]".
+  { rewrite !take_length. lia. }
+  iFrame.
+Qed.
 
-  Lemma big_sepL_merge {PROP: bi} {A: Type} (l: list A) (HNoDup: NoDup l) (φ: A -> PROP) {Haffine: forall a, Affine (φ a)}:
-    forall l1 l2, (forall a, a ∈ l -> a ∈ l1 \/ a ∈ l2) ->
-             (([∗ list] a ∈ l1, φ a) -∗
-              ([∗ list] a ∈ l2, φ a) -∗
-              ([∗ list] a ∈ l, φ a))%I.
-  Proof.
-    iInduction (l) as [|x l] "IH"; iIntros (l1 l2 H) "Hl1 Hl2".
-    - iApply big_sepL_nil; auto.
-    - iApply big_sepL_cons. destruct (H x ltac:(eapply elem_of_list_here)) as [H'|H']; eapply elem_of_list_lookup in H'; destruct H' as [k H'].
-      + iDestruct (big_sepL_delete with "Hl1") as "[$ Hl1]"; eauto.
-        iAssert ([∗ list] a ∈ delete k l1, φ a)%I with "[Hl1]" as "Hl1".
-        { iApply (big_sepL_impl with "[Hl1]"); auto.
-          iApply (big_sepL_delete' with "Hl1"). }
-        assert (Hincl: ∀ a : A, a ∈ l → a ∈ delete k l1 ∨ a ∈ l2).
-        { intros. destruct (H a ltac:(eapply elem_of_list_further; eauto)).
-          - left. eapply elem_of_list_lookup in H1. destruct H1.
-            eapply elem_of_list_lookup. assert (x0 <> k).
-            + red; intros; subst x0. rewrite H1 in H'; inversion H'.
-              inversion HNoDup. eapply H5. subst. auto.
-            + assert  (x0 < k \/ k <= x0) by lia. destruct H3.
-              * exists x0. rewrite lookup_delete_lt; auto.
-              * exists (x0 - 1). rewrite lookup_delete_ge; auto; try lia.
-                replace (S (x0 - 1)) with x0; auto. lia.
-          - right. auto. }
-        inversion HNoDup. iApply ("IH" $! H3 (delete k l1) l2 Hincl with "[$Hl1] [$Hl2]").
-      + iDestruct (big_sepL_delete with "Hl2") as "[$ Hl2]"; eauto.
-        iAssert ([∗ list] a ∈ delete k l2, φ a)%I with "[Hl2]" as "Hl2".
-        { iApply (big_sepL_impl with "[Hl2]"); auto.
-          iApply (big_sepL_delete' with "Hl2"). }
-        assert (Hincl: ∀ a : A, a ∈ l → a ∈ l1 ∨ a ∈ delete k l2).
-        { intros. destruct (H a ltac:(eapply elem_of_list_further; eauto)).
-          - left. auto.
-          - right. eapply elem_of_list_lookup in H1. destruct H1.
-            eapply elem_of_list_lookup. assert (x0 <> k).
-            + red; intros; subst x0. rewrite H1 in H'; inversion H'.
-              inversion HNoDup. subst. eapply H5. auto.
-            + assert  (x0 < k \/ k <= x0) by lia. destruct H3.
-              * exists x0. rewrite lookup_delete_lt; auto.
-              * exists (x0 - 1). rewrite lookup_delete_ge; auto; try lia.
-                replace (S (x0 - 1)) with x0; auto. lia. }
-        inversion HNoDup. iApply ("IH" $! H3 l1 (delete k l2) Hincl with "[$Hl1] [$Hl2]").
-  Qed.
+Lemma big_sepL_delete' {PROP: bi} {A: Type} (φ: A -> PROP) (l: list A):
+      forall k, (([∗ list] k0↦y ∈ l, if decide (k0 = k) then emp else φ y) -∗
+           ([∗ list] k0↦x0 ∈ delete k l, (λ (_ : nat) (x1 : A), φ x1) k0 x0))%I.
+Proof.
+  iInduction (l) as [|x l] "IH"; simpl; auto; iIntros (k) "H".
+  iDestruct "H" as "[H1 H2]".
+  rewrite /delete /=. destruct k.
+  - iApply (big_sepL_impl with "H2").
+    iClear "H1". iModIntro. iIntros. destruct (decide (S k = 0)); auto. lia.
+  - simpl. iFrame. iApply ("IH" with "[H2]").
+    iApply (big_sepL_impl with "H2").
+    iModIntro; iIntros. destruct (decide (k0 = k)); destruct (decide (S k0 = S k)); auto; lia.
+Qed.
 
-  Lemma big_sepL2_to_big_sepM (PROP : bi) (A B : Type) `{EqDecision A} `{Countable A}
-        (φ: A -> B -> PROP) (l1: list A) (l2: list B):
-        NoDup l1 ->
-        (([∗ list] y1;y2 ∈ l1;l2, φ y1 y2) -∗
-        ([∗ map] y1↦y2 ∈ list_to_map (zip l1 l2), φ y1 y2))%I.
-  Proof.
-    revert l2. iInduction (l1) as [|x l1] "IH"; iIntros (l2 Hnd) "H".
-    - iSimpl. iDestruct (big_sepL2_length with "H") as "%".
-      destruct l2; simpl in H0; inversion H0.
-      iApply big_sepM_empty. auto.
-    - iDestruct (big_sepL2_length with "H") as "%".
-      destruct l2; simpl in H0; inversion H0.
-      simpl. inversion Hnd. iDestruct "H" as "[A B]".
-      iApply (big_sepM_insert with "[A B]").
-      + eapply not_elem_of_list_to_map.
-        rewrite fst_zip; auto. lia.
-      + iFrame. iApply ("IH" $! l2 H5 with "B"); auto.
-  Qed.
+Lemma big_sepL_merge {PROP: bi} {A: Type} (l: list A) (HNoDup: NoDup l) (φ: A -> PROP) {Haffine: forall a, Affine (φ a)}:
+  forall l1 l2, (forall a, a ∈ l -> a ∈ l1 \/ a ∈ l2) ->
+           (([∗ list] a ∈ l1, φ a) -∗
+            ([∗ list] a ∈ l2, φ a) -∗
+            ([∗ list] a ∈ l, φ a))%I.
+Proof.
+  iInduction (l) as [|x l] "IH"; iIntros (l1 l2 H) "Hl1 Hl2".
+  - iApply big_sepL_nil; auto.
+  - iApply big_sepL_cons. destruct (H x ltac:(eapply elem_of_list_here)) as [H'|H']; eapply elem_of_list_lookup in H'; destruct H' as [k H'].
+    + iDestruct (big_sepL_delete with "Hl1") as "[$ Hl1]"; eauto.
+      iAssert ([∗ list] a ∈ delete k l1, φ a)%I with "[Hl1]" as "Hl1".
+      { iApply (big_sepL_impl with "[Hl1]"); auto.
+        iApply (big_sepL_delete' with "Hl1"). }
+      assert (Hincl: ∀ a : A, a ∈ l → a ∈ delete k l1 ∨ a ∈ l2).
+      { intros. destruct (H a ltac:(eapply elem_of_list_further; eauto)).
+        - left. eapply elem_of_list_lookup in H1. destruct H1.
+          eapply elem_of_list_lookup. assert (x0 <> k).
+          + red; intros; subst x0. rewrite H1 in H'; inversion H'.
+            inversion HNoDup. eapply H5. subst. auto.
+          + assert  (x0 < k \/ k <= x0) by lia. destruct H3.
+            * exists x0. rewrite lookup_delete_lt; auto.
+            * exists (x0 - 1). rewrite lookup_delete_ge; auto; try lia.
+              replace (S (x0 - 1)) with x0; auto. lia.
+        - right. auto. }
+      inversion HNoDup. iApply ("IH" $! H3 (delete k l1) l2 Hincl with "[$Hl1] [$Hl2]").
+    + iDestruct (big_sepL_delete with "Hl2") as "[$ Hl2]"; eauto.
+      iAssert ([∗ list] a ∈ delete k l2, φ a)%I with "[Hl2]" as "Hl2".
+      { iApply (big_sepL_impl with "[Hl2]"); auto.
+        iApply (big_sepL_delete' with "Hl2"). }
+      assert (Hincl: ∀ a : A, a ∈ l → a ∈ l1 ∨ a ∈ delete k l2).
+      { intros. destruct (H a ltac:(eapply elem_of_list_further; eauto)).
+        - left. auto.
+        - right. eapply elem_of_list_lookup in H1. destruct H1.
+          eapply elem_of_list_lookup. assert (x0 <> k).
+          + red; intros; subst x0. rewrite H1 in H'; inversion H'.
+            inversion HNoDup. subst. eapply H5. auto.
+          + assert  (x0 < k \/ k <= x0) by lia. destruct H3.
+            * exists x0. rewrite lookup_delete_lt; auto.
+            * exists (x0 - 1). rewrite lookup_delete_ge; auto; try lia.
+              replace (S (x0 - 1)) with x0; auto. lia. }
+      inversion HNoDup. iApply ("IH" $! H3 l1 (delete k l2) Hincl with "[$Hl1] [$Hl2]").
+Qed.
 
-  Lemma big_sepL2_bupd
-     : ∀ (PROP : bi) (H : BiBUpd PROP) (A B : Type) (Φ : A → B → PROP) (l1 : list A) (l2: list B),
-         ([∗ list] k;x ∈ l1;l2, |==> Φ k x) -∗ |==> [∗ list] k;x ∈ l1;l2, Φ k x.
-  Proof.
-    intros. revert l2. induction l1 as [| x l1].
-    { intros. iIntros "H".
-      iDestruct (big_sepL2_length with "H") as %Hlen. cbn in Hlen.
-      destruct l2; [| by inversion Hlen]. cbn. eauto. }
-    { intros. iIntros "H".
-      iDestruct (big_sepL2_length with "H") as %Hlen. cbn in Hlen.
-      destruct l2; [by inversion Hlen |]. cbn. iDestruct "H" as "[>? H]".
-      iDestruct (IHl1 with "H") as ">?". iModIntro. iFrame. }
-  Qed.
+Lemma big_sepL2_to_big_sepM (PROP : bi) (A B : Type) `{EqDecision A} `{Countable A}
+      (φ: A -> B -> PROP) (l1: list A) (l2: list B):
+      NoDup l1 ->
+      (([∗ list] y1;y2 ∈ l1;l2, φ y1 y2) -∗
+      ([∗ map] y1↦y2 ∈ list_to_map (zip l1 l2), φ y1 y2))%I.
+Proof.
+  revert l2. iInduction (l1) as [|x l1] "IH"; iIntros (l2 Hnd) "H".
+  - iSimpl. iDestruct (big_sepL2_length with "H") as "%".
+    destruct l2; simpl in H0; inversion H0.
+    iApply big_sepM_empty. auto.
+  - iDestruct (big_sepL2_length with "H") as "%".
+    destruct l2; simpl in H0; inversion H0.
+    simpl. inversion Hnd. iDestruct "H" as "[A B]".
+    iApply (big_sepM_insert with "[A B]").
+    + eapply not_elem_of_list_to_map.
+      rewrite fst_zip; auto. lia.
+    + iFrame. iApply ("IH" $! l2 H5 with "B"); auto.
+Qed.
+
+Lemma big_sepL2_bupd
+   : ∀ (PROP : bi) (H : BiBUpd PROP) (A B : Type) (Φ : A → B → PROP) (l1 : list A) (l2: list B),
+       ([∗ list] k;x ∈ l1;l2, |==> Φ k x) -∗ |==> [∗ list] k;x ∈ l1;l2, Φ k x.
+Proof.
+  intros. revert l2. induction l1 as [| x l1].
+  { intros. iIntros "H".
+    iDestruct (big_sepL2_length with "H") as %Hlen. cbn in Hlen.
+    destruct l2; [| by inversion Hlen]. cbn. eauto. }
+  { intros. iIntros "H".
+    iDestruct (big_sepL2_length with "H") as %Hlen. cbn in Hlen.
+    destruct l2; [by inversion Hlen |]. cbn. iDestruct "H" as "[>? H]".
+    iDestruct (IHl1 with "H") as ">?". iModIntro. iFrame. }
+Qed.
+
+(* Helper lemma for reasoning about the current state of a region map *)
+Lemma big_sepM_exists `{Σ : gFunctors} {A B C : Type} `{EqDecision A, Countable A} (m : gmap A B) (φ : A → C -> B → iProp Σ) :
+  (([∗ map] a↦b ∈ m, ∃ c, φ a c b) ∗-∗ (∃ (m' : gmap A C), [∗ map] a↦c;b ∈ m';m, φ a c b))%I.
+Proof.
+  iSplit.
+  - iIntros "Hmap".
+    iInduction (m) as [| a x m Hnone] "IH" using map_ind.
+    + iExists empty. done.
+    + iDestruct (big_sepM_insert with "Hmap") as "[Hc Hmap]"; auto.
+      iDestruct "Hc" as (c) "Hc".
+      iDestruct ("IH" with "Hmap") as (m') "Hmap".
+      iExists (<[a:=c]> m').
+      iApply (big_sepM2_insert_2 with "Hc").
+      iFrame.
+  - iIntros "Hmap".
+    iDestruct "Hmap" as (m') "Hmap".
+    iInduction (m) as [| a x m Hnone] "IH" using map_ind forall (m').
+    + done.
+    + iDestruct (big_sepM2_dom with "Hmap") as %Hdom.
+      assert (is_Some (m' !! a)) as [ρ Hρ].
+      { apply elem_of_gmap_dom. rewrite Hdom dom_insert_L.
+        apply elem_of_union_l, elem_of_singleton; auto. }
+      rewrite -(insert_id m' a ρ); auto.
+      rewrite -insert_delete.
+      iDestruct (big_sepM2_insert with "Hmap") as "[Hφ Hmap]";[apply lookup_delete|auto|].
+      iApply big_sepM_insert;auto.
+      iDestruct ("IH" with "Hmap") as "Hmap". iFrame.
+      iExists ρ. iFrame.
+Qed.
